Add theory about "horizontal" ... ????

proof/Preservation.v
@@ -201,8 +201,105 @@ Proof.
     etrans; eauto.
 Qed.
 
-Inductive local_preservation_excl (sound_state: Sound.t -> ms.(state) -> Prop): Prop :=
-| local_preservation_excl_intro
+Inductive local_preservation_strong_horizontal (sound_state: Sound.t -> ms.(state) -> Prop): Prop :=
+| local_preservation_strong_horizontal_intro
+    (INIT: forall
+        su_arg args st_init
+        (SUARG: Sound.args su_arg args)
+        (SKENV: Sound.skenv su_arg args.(Args.m) ms.(ModSem.skenv))
+        (INIT: ms.(ModSem.initial_frame) args st_init)
+      ,
+        exists su_init, (<<LE: Sound.le su_arg su_init>>) /\
+                        (<<SUST: sound_state su_init st_init>>)
+                        /\ (<<MLE: su_init.(Sound.mle) args.(Args.m) st_init.(get_mem)>>))
+    (STEP: forall
+        su0 st0 tr st1
+        (SUST: sound_state su0 st0)
+        (SAFE: ~ ms.(ModSem.is_call) st0 /\ ~ ms.(ModSem.is_return) st0)
+        (STEP: Step ms st0 tr st1)
+      ,
+        (* <<SUST: sound_state su0 st1>> /\ <<MLE: su0.(Sound.mle) st0.(get_mem) st1.(get_mem)>>) *)
+        exists su1, <<LE: Sound.le su0 su1>> /\ <<SUST: sound_state su1 st1>> /\ <<MLE: su0.(Sound.mle) st0.(get_mem) st1.(get_mem)>>)
+    (CALL: forall
+        su0 st0 args
+        (SUST: sound_state su0 st0)
+        (AT: ms.(ModSem.at_external) st0 args)
+      ,
+        <<MLE: Sound.mle su0 st0.(get_mem) args.(Args.m)>> /\
+        exists su_gr,
+          (<<GR: Sound.get_greatest su0 args su_gr>>) /\
+          (* (<<LE: Sound.le su0 su_lifted>>) /\ *)
+          (* (<<ARGS: su_lifted.(Sound.args) args>>) /\ *)
+          (<<K: forall
+              su_ret retv st1
+              (LE: Sound.le su_gr su_ret)
+              (RETV: su_ret.(Sound.retv) retv)
+              (* retv st1 *)
+              (* (RETV: su_gr.(Sound.retv) retv) *)
+              (MLE: Sound.mle su_gr args.(Args.m) retv.(Retv.m))
+              (AFTER: ms.(ModSem.after_external) st0 retv st1)
+            ,
+              exists su1,
+                <<LE: Sound.le su_ret su1>> /\
+              (* (<<SUST: sound_state su0 args.(Args.m) st1>>)>>)) *)
+              (* (<<SUST: sound_state su0 st1>> /\ <<MLE: su0.(Sound.mle) st0.(get_mem) st1.(get_mem)>>)>>)) *)
+              (<<SUST: sound_state su1 st1>> /\ <<MLE: su0.(Sound.mle) retv.(Retv.m) st1.(get_mem)>>)>>))
+    (RET: forall
+        su0 st0 retv
+        (SUST: sound_state su0 st0)
+        (FINAL: ms.(ModSem.final_frame) st0 retv)
+      ,
+        exists su_ret, <<LE: Sound.le su0 su_ret>> /\
+        <<RETV: su_ret.(Sound.retv) retv>> /\ <<MLE: su0.(Sound.mle) st0.(get_mem) retv.(Retv.m)>>)
+.
+
+Theorem local_preservation_strong_horizontal_spec
+        sound_state
+        (PRSV: local_preservation_strong_horizontal sound_state)
+  :
+    <<PRSV: local_preservation (fun su m_init st =>
+                                  <<MLE: su.(Sound.mle) m_init st.(get_mem)>> /\
+                                  exists su_h,
+                                    <<LE: Sound.le su su_h>> /\ sound_state su_h st)>>
+.
+Proof.
+  inv PRSV.
+  econs; eauto.
+  - ii. exploit INIT; eauto. i; des. esplits; eauto. eapply Sound.le_spec; eauto.
+  - ii. des. exploit STEP; eauto. i; des. esplits; try apply SUST; eauto.
+    + etrans; eauto.
+      eapply Sound.le_spec; eauto.
+    + etrans; eauto.
+  - ii. des. exploit CALL; eauto. i; des.
+    assert(exists su_grh, <<GRH: Sound.get_greatest su0 args su_grh>>).
+    { exploit Sound.greatest_adq; eauto. i; des.
+      exploit (Sound.greatest_ex su0); eauto.
+      { esplits; try apply SUARGS; eauto. etrans; eauto. }
+    }
+    des.
+    assert(su_grh = su_gr).
+    { admit "ValueAnalysisC - irr". }
+    clarify.
+    assert(LE1: Sound.le su_h su_gr).
+    { eapply Sound.greatest_adq; eauto. }
+    esplits; eauto.
+    { etrans; eauto.
+      + eapply Sound.le_spec; eauto.
+    }
+    ii. exploit K; eauto. i; des. esplits; try apply SUST; eauto.
+    + etrans; eauto.
+      eapply Sound.le_spec; eauto.
+      etrans; eauto.
+      etrans; eauto.
+      eapply Sound.le_spec; eauto.
+    + etrans; eauto. etrans; eauto. etrans; eauto.
+  - ii; des. exploit RET; eauto. i; des. esplits; try apply RETV; eauto.
+    + etrans; eauto.
+    + etrans; eauto. eapply Sound.le_spec; eauto.
+Qed.
+
+Inductive local_preservation_strong_excl (sound_state: Sound.t -> ms.(state) -> Prop): Prop :=
+| local_preservation_strong_excl_intro
     (has_footprint: ms.(state) -> mem -> Prop) (mle_excl: ms.(state) -> Sound.t -> mem -> mem -> Prop)
     (FOOTLE: forall
         su0 st_at m0 m1
@@ -256,9 +353,9 @@ Inductive local_preservation_excl (sound_state: Sound.t -> ms.(state) -> Prop): 
         <<RETV: su_ret.(Sound.retv) retv>> /\ <<MLE: su0.(Sound.mle) st0.(get_mem) retv.(Retv.m)>>)
 .
 
-Theorem local_preservation_excl_spec
+Theorem local_preservation_strong_excl_spec
         sound_state
-        (PRSV: local_preservation_excl sound_state)
+        (PRSV: local_preservation_strong_excl sound_state)
   :
     <<PRSV: local_preservation (fun su m_init st => sound_state su st /\ su.(Sound.mle) m_init st.(get_mem))>>
 .
@@ -275,6 +372,119 @@ Proof.
     eapply FOOTLE; eauto.
   - ii; des. exploit RET; eauto. i; des. esplits; eauto.
     etrans; eauto.
+Qed.
+
+Inductive local_preservation_strong_horizontal_excl (sound_state: Sound.t -> ms.(state) -> Prop): Prop :=
+| local_preservation_strong_horizontal_excl_intro
+    (has_footprint: ms.(state) -> mem -> Prop) (mle_excl: ms.(state) -> Sound.t -> mem -> mem -> Prop)
+    (FOOTLE: forall
+        su0 st_at m0 m1
+        (FOOT: has_footprint st_at m0)
+        (MLE: su0.(Sound.mle) m0 m1)
+      ,
+        <<FOOT: has_footprint st_at m1>>)
+    (FOOTWEAK: forall
+        su0 st_at m0 m1
+        (FOOT: has_footprint st_at m0)
+        (MLE: (mle_excl st_at) su0 m0 m1)
+      ,
+        <<MLE: Sound.mle su0 m0 m1>>)
+    (INIT: forall
+        su_arg args st_init
+        (SUARG: Sound.args su_arg args)
+        (SKENV: Sound.skenv su_arg args.(Args.m) ms.(ModSem.skenv))
+        (INIT: ms.(ModSem.initial_frame) args st_init)
+      ,
+        exists su_init, (<<LE: Sound.le su_arg su_init>>) /\
+                        (<<SUST: sound_state su_init st_init>>)
+                        /\ (<<MLE: su_init.(Sound.mle) args.(Args.m) st_init.(get_mem)>>))
+    (STEP: forall
+        su0 st0 tr st1
+        (SUST: sound_state su0 st0)
+        (SAFE: ~ ms.(ModSem.is_call) st0 /\ ~ ms.(ModSem.is_return) st0)
+        (STEP: Step ms st0 tr st1)
+      ,
+        (* <<SUST: sound_state su0 st1>> /\ <<MLE: su0.(Sound.mle) st0.(get_mem) st1.(get_mem)>>) *)
+        exists su1, <<LE: Sound.le su0 su1>> /\ <<SUST: sound_state su1 st1>> /\ <<MLE: su0.(Sound.mle) st0.(get_mem) st1.(get_mem)>>)
+    (CALL: forall
+        su0 st0 args
+        (SUST: sound_state su0 st0)
+        (AT: ms.(ModSem.at_external) st0 args)
+      ,
+        <<MLE: Sound.mle su0 st0.(get_mem) args.(Args.m)>> /\
+        <<FOOT: has_footprint st0 args.(Args.m)>> /\
+        exists su_gr,
+          (<<GR: Sound.get_greatest su0 args su_gr>>) /\
+          (* (<<LE: Sound.le su0 su_lifted>>) /\ *)
+          (* (<<ARGS: su_lifted.(Sound.args) args>>) /\ *)
+          (<<K: forall
+              su_ret retv st1
+              (LE: Sound.le su_gr su_ret)
+              (RETV: su_ret.(Sound.retv) retv)
+              (* retv st1 *)
+              (* (RETV: su_gr.(Sound.retv) retv) *)
+              (MLE: Sound.mle su_gr args.(Args.m) retv.(Retv.m))
+              (AFTER: ms.(ModSem.after_external) st0 retv st1)
+            ,
+              exists su1,
+                <<LE: Sound.le su_ret su1>> /\
+              (* (<<SUST: sound_state su0 args.(Args.m) st1>>)>>)) *)
+              (* (<<SUST: sound_state su0 st1>> /\ <<MLE: su0.(Sound.mle) st0.(get_mem) st1.(get_mem)>>)>>)) *)
+              (<<SUST: sound_state su1 st1>> /\ <<MLE: (mle_excl st0) su0 retv.(Retv.m) st1.(get_mem)>>)>>))
+    (RET: forall
+        su0 st0 retv
+        (SUST: sound_state su0 st0)
+        (FINAL: ms.(ModSem.final_frame) st0 retv)
+      ,
+        exists su_ret, <<LE: Sound.le su0 su_ret>> /\
+        <<RETV: su_ret.(Sound.retv) retv>> /\ <<MLE: su0.(Sound.mle) st0.(get_mem) retv.(Retv.m)>>)
+.
+
+Theorem local_preservation_strong_horizontal_excl_spec
+        sound_state
+        (PRSV: local_preservation_strong_horizontal_excl sound_state)
+  :
+    <<PRSV: local_preservation (fun su m_init st =>
+                                  <<MLE: su.(Sound.mle) m_init st.(get_mem)>> /\
+                                  exists su_h,
+                                    <<LE: Sound.le su su_h>> /\ sound_state su_h st)>>
+.
+Proof.
+  inv PRSV.
+  econs; eauto.
+  - ii. exploit INIT; eauto. i; des. esplits; eauto. eapply Sound.le_spec; eauto.
+  - ii. des. exploit STEP; eauto. i; des. esplits; try apply SUST; eauto.
+    + etrans; eauto.
+      eapply Sound.le_spec; eauto.
+    + etrans; eauto.
+  - ii. des. exploit CALL; eauto. i; des.
+    assert(exists su_grh, <<GRH: Sound.get_greatest su0 args su_grh>>).
+    { exploit Sound.greatest_adq; eauto. i; des.
+      exploit (Sound.greatest_ex su0); eauto.
+      { esplits; try apply SUARGS; eauto. etrans; eauto. }
+    }
+    des.
+    assert(su_grh = su_gr).
+    { admit "ValueAnalysisC - irr". }
+    clarify.
+    assert(LE1: Sound.le su_h su_gr).
+    { eapply Sound.greatest_adq; eauto. }
+    esplits; eauto.
+    { etrans; eauto.
+      + eapply Sound.le_spec; eauto.
+    }
+    ii. exploit K; eauto. i; des. esplits; try apply SUST; eauto.
+    + etrans; eauto.
+      eapply Sound.le_spec; eauto.
+      etrans; eauto.
+      etrans; eauto.
+      * eapply Sound.le_spec; eauto.
+      * eapply FOOTWEAK; eauto.
+        eapply FOOTLE; eauto.
+    + etrans; eauto. etrans; eauto. etrans; eauto.
+  - ii; des. exploit RET; eauto. i; des. esplits; try apply RETV; eauto.
+    + etrans; eauto.
+    + etrans; eauto. eapply Sound.le_spec; eauto.
 Qed.
 
 End PRSV.
